MSet/MMapWeakList.v
@@ -1,0 +1,705 @@
+(***********************************************************************)
+(*  v      *   The Coq Proof Assistant  /  The Coq Development Team    *)
+(* <O___,, *        INRIA-Rocquencourt  &  LRI-CNRS-Orsay              *)
+(*   \VV/  *************************************************************)
+(*    //   *      This file is distributed under the terms of the      *)
+(*         *       GNU Lesser General Public License Version 2.1       *)
+(***********************************************************************)
+
+(** * Finite sets library *)
+
+(** This file proposes an implementation of the non-dependant
+    interface [MSetWeakInterface.S] using lists without redundancy. *)
+
+Require Import MMapInterface.
+Set Implicit Arguments.
+Unset Strict Implicit.
+
+(** * Functions over lists
+
+   First, we provide sets as lists which are (morally) without redundancy.
+   The specs are proved under the additional condition of no redundancy.
+   And the functions returning sets are proved to preserve this invariant. *)
+
+
+(** ** The set operations. *)
+
+Module Ops (X: DecidableType) <: WOps X.
+
+  Definition key := X.t.
+
+  Section Foo.
+  Variable A : Type.
+
+  Definition t  := list (key * A).
+
+  Definition empty : t := nil.
+
+  Definition is_empty (l : t) : bool := if l then true else false.
+
+  Fixpoint mem (x : key) (s : t) : bool :=
+    match s with
+    | nil => false
+    | (k, v) :: l =>
+           if X.eq_dec x k then true else mem x l
+    end.
+
+  Fixpoint find (x : key) (s : t) : option A :=
+    match s with
+    | nil => None
+    | (k, v) :: l =>
+           if X.eq_dec x k then Some v else find x l
+    end.
+
+  Fixpoint add (x : key) (v : A) (s : t) : t :=
+    match s with
+    | nil => (x, v) :: nil
+    | (y, v) :: l =>
+        if X.eq_dec x y then s else (y, v) :: add x v l
+    end.
+
+  Definition singleton (x : key) (v : A) : t := (x, v) :: nil.
+
+  Fixpoint remove (x : key) (s : t) : t :=
+    match s with
+    | nil => nil
+    | (y, v) :: l =>
+        if X.eq_dec x y then l else (y, v) :: remove x l
+    end.
+
+  Definition fold (B : Type) (f : key -> A -> B -> B) (s : t) (i : B) : B :=
+    fold_left (fun a p => f (fst p) (snd p) a) s i.
+
+  (*
+  Definition union (s : t) : t -> t := fold add s.
+
+  Definition diff (s s' : t) : t := fold (fun k v => remove k) s' s.
+
+  Definition inter (s s': t) : t :=
+    fold (fun x k s => if mem x s' then add x k s else s) s nil.
+   *)
+ 
+  Fixpoint filter (f : key -> A -> bool) (s : t) : t :=
+    match s with
+    | nil => nil
+    | (x, v) :: l => if f x v then (x, v) :: filter f l else filter f l
+    end.
+
+  Fixpoint for_all (f : key -> A -> bool) (s : t) : bool :=
+    match s with
+    | nil => true
+    | (x, v) :: l => if f x v then for_all f l else false
+    end.
+
+  Section ElemEq.
+  Variable eq : A -> A -> bool.
+
+  Definition subset (s s' : t) : bool :=
+    for_all (fun k v =>
+               match find k s' with
+               | Some v' => eq v v'
+               | None => false end) s.
+
+  Definition equal (s s' : t) : bool := andb (subset s s') (subset s' s).
+  End ElemEq.
+
+  Fixpoint exists_ (f : key -> A -> bool) (s : t) : bool :=
+    match s with
+    | nil => false
+    | (x, v) :: l => if f x v then true else exists_ f l
+    end.
+
+  Fixpoint partition (f : key -> A -> bool) (s : t) : t * t :=
+    match s with
+    | nil => (nil, nil)
+    | (x, v) :: l =>
+        let (s1, s2) := partition f l in
+        if f x v then ((x,v) :: s1, s2) else (s1, (x,v) :: s2)
+    end.
+
+  Definition cardinal (s : t) : nat := length s.
+
+  Definition elements (s : t) : list (key * A) := s.
+
+  Definition choose (s : t) : option (key * A) :=
+     match s with
+      | nil => None
+      | x::_ => Some x
+     end.
+  End Foo.
+End Ops.
+
+(** ** Proofs of set operation specifications. *)
+
+Module MakeRaw (X:DecidableType) <: WRawMaps X.
+  Include Ops X.
+
+  Section ForNotations.
+  Variable A : Type.
+
+  Inductive MapsToA (x : key) (v : A) : t A -> Prop :=
+  | MapsTo_cons_hd : forall k l, X.eq x k -> MapsToA x v ((k,v) :: l)
+  | MapsTo_cons_tl : forall k v' l, MapsToA x v l -> MapsToA x v ((k,v') :: l).
+
+  Definition MapsTo := MapsToA.
+  Definition In (k:key) (m: t A) : Prop := exists e:A, MapsTo k e m.
+  Inductive NoDup : t A -> Prop :=
+  | NoDup_nil : NoDup nil
+  | NoDup_cons : forall x v l, ~ In x l -> NoDup l -> NoDup ((x,v)::l).
+
+  (* TODO: modify proofs in order to avoid these hints *)
+  Let eqr:= (@Equivalence_Reflexive _ _ X.eq_equiv).
+  Let eqsym:= (@Equivalence_Symmetric _ _ X.eq_equiv).
+  Let eqtrans:= (@Equivalence_Transitive _ _ X.eq_equiv).
+  Hint Resolve eqr eqtrans.
+  Hint Immediate eqsym.
+
+  Definition IsOk := NoDup.
+
+  Class Ok (s:t A) : Prop := ok : NoDup s.
+
+  Hint Unfold Ok.
+  Hint Resolve ok.
+
+  Instance NoDup_Ok s (nd : NoDup s) : Ok s := { ok := nd }.
+
+  Ltac inv_ok := match goal with
+   | H:Ok (_ :: _) |- _ => inversion_clear H; inv_ok
+   | H:Ok nil |- _ => clear H; inv_ok
+   | H:NoDup ?l |- _ => change (Ok l) in H; inv_ok
+   | _ => idtac
+  end.
+
+  Ltac inv := invlist InA; inv_ok.
+  Ltac constructors := repeat constructor.
+
+  Fixpoint memA (x : key) (l : t A) := match l with
+   | nil => false
+   | (k,v)::l => if X.eq_dec x k then true else memA x l
+  end.
+
+  Fixpoint isok l := match l with
+   | nil => true
+   | (x,v)::l => negb (memA x l) && isok l
+  end.
+
+  Definition Equal m m' := forall k, @find A k m = find k m'.
+  Definition Equiv (eq_elt: A -> A -> Prop) m m' :=
+         (forall k, In k m <-> In k m') /\
+         (forall k e e', MapsTo k e m -> MapsTo k e' m' -> eq_elt e e').
+  Definition Equivb (cmp: A -> A -> bool) := Equiv (Cmp cmp).
+
+  Definition Empty s := forall a : key, ~ In a s.
+  Definition For_all (P : key -> A -> Prop) s := forall x a, MapsTo x a s -> P x a.
+  Definition Exists (P : key -> A -> Prop) s := exists x a, MapsTo x a s /\ P x a.
+
+
+  Lemma In_compat : Proper (X.eq==>eq==>iff) In.
+  Proof.
+  repeat red; intros. subst. (* rewrite H; auto.*) admit.
+  Qed.
+
+  Lemma mem_spec : forall s x `{Ok s},
+   mem x s = true <-> In x s.
+  Proof.
+  (*
+  intros. induction H.
+  split; intros; inv. discriminate. inversion H. inversion H0.
+
+  split; intros; inv; auto.
+  *)
+
+  (*
+  induction s; intros.
+  split; intros; inv. discriminate.
+  simpl; destruct (X.eq_dec x a); split; intros; inv; auto.
+  right; rewrite <- IHs; auto.
+  rewrite IHs; auto.
+  Qed.
+  *)
+  Admitted.
+
+  Lemma isok_iff : forall l, Ok l <-> isok l = true.
+  Proof.
+    (*
+  induction l.
+  intuition.
+  simpl.
+  rewrite andb_true_iff.
+  rewrite negb_true_iff.
+  rewrite <- IHl.
+  split; intros H. inv.
+  split; auto.
+  apply not_true_is_false. rewrite mem_spec; auto.
+  destruct H; constructors; auto.
+  rewrite <- mem_spec; auto; congruence.
+  Qed.
+     *)
+  Admitted.
+
+  Global Instance isok_Ok l : isok l = true -> Ok l | 10.
+  Proof.
+    (*
+  intros. apply <- isok_iff; auto.
+  Qed.
+    *)
+  Admitted.
+
+  Lemma add_spec1: forall s k k' v `{Ok s},
+     X.eq k k' -> MapsTo k v (add k' v s).
+  Admitted.
+  
+  Lemma add_spec2: forall s k k' v v' `{Ok s},
+     ~ X.eq k k' -> (MapsTo k v (add k' v' s) <-> MapsTo k v s).
+  Admitted.
+
+  (*
+  Lemma add_spec :
+   forall (s : t A) (x y : key) {Hs : Ok s},
+     In y (add x s) <-> X.eq y x \/ In y s.
+  Proof.
+  induction s; simpl; intros.
+  intuition; inv; auto.
+  destruct X.eq_dec; inv; rewrite InA_cons, ?IHs; intuition.
+  left; eauto.
+  inv; auto.
+  Qed.
+  *)
+
+  Global Instance add_ok s k v `(Ok s) : Ok (add k v s).
+  (*
+  Proof.
+  induction s.
+  simpl; intuition.
+  intros; inv. simpl.
+  destruct X.eq_dec; auto.
+  constructors; auto.
+  intro; inv; auto.
+  rewrite add_spec in *; intuition.
+  Qed.
+  *)
+  Admitted.
+
+  Lemma remove_spec :
+   forall (s : t A) (x y : key) {Hs : Ok s},
+     In y (remove x s) <-> In y s /\ ~X.eq y x.
+  Admitted.
+  (*
+  Proof.
+  induction s; simpl; intros.
+  intuition; inv; auto.
+  destruct X.eq_dec; inv; rewrite !InA_cons, ?IHs; intuition.
+  elim H. setoid_replace a with y; eauto.
+  elim H3. setoid_replace x with y; eauto.
+  elim n. eauto.
+  Qed.
+  *)
+
+  Global Instance remove_ok s x `(Ok s) : Ok (remove x s).
+  Admitted.
+  (*
+  Proof.
+  induction s; simpl; intros.
+  auto.
+  destruct X.eq_dec; inv; auto.
+  constructors; auto.
+  rewrite remove_spec; intuition.
+  Qed.
+  *)
+
+  Lemma singleton_ok : forall k v, Ok (singleton k v).
+  Proof.
+  intros.
+  unfold singleton, Ok. constructors. unfold In. intro.
+  inversion H. inversion H0.
+  Qed.
+
+  Lemma singleton_spec : forall k k' v,
+    X.eq k k' <-> MapsTo k v (singleton k' v).
+  Admitted.
+
+
+  (*
+  Lemma singleton_spec : forall x y : elt, In y (singleton x) <-> X.eq y x.
+  Proof.
+  unfold singleton; simpl; split; intros. inv; auto. left; auto.
+  Qed.
+  *)
+
+  Lemma empty_ok : Ok (empty A).
+  Proof.
+  unfold empty; constructors.
+  Qed.
+
+  Lemma empty_spec : Empty (empty A).
+  Proof.
+  unfold Empty, empty; red; intros; inv.
+  unfold In in H. inversion H. inversion H0.
+  Qed.
+
+  Lemma is_empty_spec : forall s : t A, is_empty s = true <-> Empty s.
+  Proof.
+  unfold Empty; destruct s; simpl; split; intros; auto.
+  intro; inv. unfold In in H. inversion H. inversion H0. inversion H1. inversion H.
+  assert (In (fst p) (p :: s)).
+    destruct p.  unfold In. exists a. constructor.
+    auto.
+  apply H in H0. inversion H0.
+  Qed.
+
+  (*
+  Lemma elements_spec1 : forall (s : t) (x : elt), In x (elements s) <-> In x s.
+  Proof.
+  unfold elements; intuition.
+  Qed.
+
+  Lemma elements_spec2w : forall (s : t) {Hs : Ok s}, NoDup (elements s).
+  Proof.
+  unfold elements; auto.
+  Qed.
+  *)
+
+  Lemma fold_spec : forall s (X : Type) (i : X) (f : key -> A -> X -> X),
+    fold f s i = fold_left (fun (x:X) (p:key*A) => f (fst p) (snd p) x ) (elements s) i.
+  Admitted.                          
+
+  (*
+  Lemma fold_spec :
+   forall (s : t) (A : Type) (i : A) (f : elt -> A -> A),
+   fold f s i = fold_left (flip f) (elements s) i.
+  Proof.
+  reflexivity.
+  Qed.
+
+  Global Instance union_ok : forall s s' `(Ok s, Ok s'), Ok (union s s').
+  Proof.
+  induction s; simpl; auto; intros; inv; unfold flip; auto with *.
+  Qed.
+
+  Lemma union_spec :
+   forall (s s' : t) (x : elt) {Hs : Ok s} {Hs' : Ok s'},
+   In x (union s s') <-> In x s \/ In x s'.
+  Proof.
+  induction s; simpl in *; unfold flip; intros; auto; inv.
+  intuition; inv.
+  rewrite IHs, add_spec, InA_cons; intuition.
+  Qed.
+
+  Global Instance inter_ok s s' `(Ok s, Ok s') : Ok (inter s s').
+  Proof.
+  unfold inter, fold, flip.
+  set (acc := nil (A:=elt)).
+  assert (Hacc : Ok acc) by constructors.
+  clearbody acc; revert acc Hacc.
+  induction s; simpl; auto; intros. inv.
+  apply IHs; auto.
+  destruct (mem a s'); auto with *.
+  Qed.
+
+  Lemma inter_spec  :
+   forall (s s' : t) (x : elt) {Hs : Ok s} {Hs' : Ok s'},
+   In x (inter s s') <-> In x s /\ In x s'.
+  Proof.
+  unfold inter, fold, flip; intros.
+  set (acc := nil (A:=elt)) in *.
+  assert (Hacc : Ok acc) by constructors.
+  assert (IFF : (In x s /\ In x s') <-> (In x s /\ In x s') \/ In x acc).
+   intuition; unfold acc in *; inv.
+  rewrite IFF; clear IFF. clearbody acc.
+  revert acc Hacc x s' Hs Hs'.
+  induction s; simpl; intros.
+  intuition; inv.
+  inv.
+  case_eq (mem a s'); intros Hm.
+  rewrite IHs, add_spec, InA_cons; intuition.
+  rewrite mem_spec in Hm; auto.
+  left; split; auto. rewrite H1; auto.
+  rewrite IHs, InA_cons; intuition.
+  rewrite H2, <- mem_spec in H3; auto. congruence.
+  Qed.
+
+  Global Instance diff_ok : forall s s' `(Ok s, Ok s'), Ok (diff s s').
+  Proof.
+  unfold diff; intros s s'; revert s.
+  induction s'; simpl; unfold flip; auto; intros. inv; auto with *.
+  Qed.
+
+  Lemma diff_spec  :
+   forall (s s' : t) (x : elt) {Hs : Ok s} {Hs' : Ok s'},
+   In x (diff s s') <-> In x s /\ ~In x s'.
+  Proof.
+  unfold diff; intros s s'; revert s.
+  induction s'; simpl; unfold flip.
+  intuition; inv.
+  intros. inv.
+  rewrite IHs', remove_spec, InA_cons; intuition.
+  Qed.
+
+  Lemma subset_spec :
+   forall (s s' : t) {Hs : Ok s} {Hs' : Ok s'},
+   subset s s' = true <-> Subset s s'.
+  Proof.
+  unfold subset, Subset; intros.
+  rewrite is_empty_spec.
+  unfold Empty; intros.
+  intuition.
+  specialize (H a). rewrite diff_spec in H; intuition.
+  rewrite <- (mem_spec a) in H |- *. destruct (mem a s'); intuition.
+  rewrite diff_spec in H0; intuition.
+  Qed.
+
+  *)
+
+ Section EqSpec.
+     Variable s s' : t A.
+     Variable cmp : A -> A -> bool.
+     Lemma equal_1 : 
+       forall `{Ok s, Ok s'},
+       Equivb cmp s s' -> equal cmp s s' = true.
+     Admitted.
+     Lemma equal_2 :
+       forall `{Ok s, Ok s'},
+       equal cmp s s' = true -> Equivb cmp s s'.
+     Admitted.
+  End EqSpec. 
+
+  (*
+
+  Lemma equal_spec :
+   forall (s s' : t) {Hs : Ok s} {Hs' : Ok s'},
+   equal s s' = true <-> Equal s s'.
+  Proof.
+  unfold Equal, equal; intros.
+  rewrite andb_true_iff, !subset_spec.
+  unfold Subset; intuition. rewrite <- H; auto. rewrite H; auto.
+  Qed.
+
+  Definition choose_spec1 :
+    forall (s : t) (x : elt), choose s = Some x -> In x s.
+  Proof.
+  destruct s; simpl; intros; inversion H; auto.
+  Qed.
+
+  Definition choose_spec2 : forall s : t, choose s = None -> Empty s.
+  Proof.
+  destruct s; simpl; intros.
+  intros x H0; inversion H0.
+  inversion H.
+  Qed.
+  *)
+ 
+  Lemma cardinal_spec : forall s `{Ok s}, cardinal s = length (elements s).
+  Proof. auto. Qed.
+
+  (*
+  Lemma filter_spec' : forall s x f,
+   In x (filter f s) -> In x s.
+  Proof.
+  induction s; simpl.
+  intuition; inv.
+  intros; destruct (f a); inv; intuition; right; eauto.
+  Qed.
+  *)
+
+  Lemma filter_spec : forall s k v f,
+    Proper (X.eq==>Logic.eq==>Logic.eq) f ->
+    (MapsTo k v (filter f s) <-> MapsTo k v s /\ f k v = true).
+  Admitted.
+
+  (*
+  Lemma filter_spec :
+   forall (s : t) (x : elt) (f : elt -> bool),
+   Proper (X.eq==>eq) f ->
+   (In x (filter f s) <-> In x s /\ f x = true).
+  Proof.
+  induction s; simpl.
+  intuition; inv.
+  intros.
+  destruct (f a) eqn:E; rewrite ?InA_cons, IHs; intuition.
+  setoid_replace x with a; auto.
+  setoid_replace a with x in E; auto. congruence.
+  Qed.
+  *)
+
+  Global Instance filter_ok s f `(Ok s) : Ok (filter f s).
+  Admitted.
+  (*
+  Proof.
+  induction s; simpl.
+  auto.
+  intros; inv.
+  case (f a); auto.
+  constructors; auto.
+  contradict H0.
+  eapply filter_spec'; eauto.
+  Qed.
+  *)
+
+  Lemma for_all_spec : forall s f,
+    Proper (X.eq==>Logic.eq==>Logic.eq) f ->
+    (for_all f s = true <-> For_all (fun x a => f x a = true) s).
+  Admitted.
+
+  (*
+  Lemma for_all_spec :
+   forall (s : t) (f : elt -> bool),
+   Proper (X.eq==>eq) f ->
+   (for_all f s = true <-> For_all (fun x => f x = true) s).
+  Proof.
+  unfold For_all; induction s; simpl.
+  intuition. inv.
+  intros; inv.
+  destruct (f a) eqn:F.
+  rewrite IHs; intuition. inv; auto.
+  setoid_replace x with a; auto.
+  split; intros H'; try discriminate.
+  intros.
+  rewrite <- F, <- (H' a); auto.
+  Qed.
+  *)
+
+  Lemma  exists_spec : forall s f ,
+    Proper (X.eq==>Logic.eq==>Logic.eq) f ->
+    (exists_ f s = true <-> Exists (fun x a => f x a = true) s).
+  Admitted.
+
+  (*
+  Lemma exists_spec :
+   forall (s : t) (f : elt -> bool),
+   Proper (X.eq==>eq) f ->
+   (exists_ f s = true <-> Exists (fun x => f x = true) s).
+  Proof.
+  unfold Exists; induction s; simpl.
+  split; [discriminate| intros (x & Hx & _); inv].
+  intros.
+  destruct (f a) eqn:F.
+  split; auto.
+  exists a; auto.
+  rewrite IHs; firstorder.
+  inv.
+  setoid_replace a with x in F; auto; congruence.
+  exists x; auto.
+  Qed.
+  *)
+
+  Lemma partition_spec1 : forall s f,
+    Proper (X.eq==>Logic.eq==>Logic.eq) f ->
+    Equal (fst (partition f s)) (filter f s).
+  Admitted.
+
+  (*
+  Lemma partition_spec1 :
+   forall (s : t) (f : elt -> bool),
+   Proper (X.eq==>eq) f ->
+   Equal (fst (partition f s)) (filter f s).
+  Proof.
+  simple induction s; simpl; auto; unfold Equal.
+  firstorder.
+  intros x l Hrec f Hf.
+  generalize (Hrec f Hf); clear Hrec.
+  case (partition f l); intros s1 s2; simpl; intros.
+  case (f x); simpl; firstorder; inversion H0; intros; firstorder.
+  Qed.
+  *)
+
+  Lemma partition_spec2 : forall s f,
+    Proper (X.eq==>Logic.eq==>Logic.eq) f ->
+    Equal (snd (partition f s)) (filter (fun x a => negb (f x a)) s).
+  Admitted.
+
+  (*
+  Lemma partition_spec2 :
+   forall (s : t) (f : elt -> bool),
+   Proper (X.eq==>eq) f ->
+   Equal (snd (partition f s)) (filter (fun x => negb (f x)) s).
+  Proof.
+  simple induction s; simpl; auto; unfold Equal.
+  firstorder.
+  intros x l Hrec f Hf.
+  generalize (Hrec f Hf); clear Hrec.
+  case (partition f l); intros s1 s2; simpl; intros.
+  case (f x); simpl; firstorder; inversion H0; intros; firstorder.
+  Qed.
+  *)
+  
+  (*
+  Lemma partition_ok1' :
+   forall (s : t) {Hs : Ok s} (f : elt -> bool)(x:elt),
+    In x (fst (partition f s)) -> In x s.
+  Proof.
+  induction s; simpl; auto; intros. inv.
+  generalize (IHs H1 f x).
+  destruct (f a); destruct (partition f s); simpl in *; auto.
+  inversion_clear H; auto.
+  Qed.
+
+  Lemma partition_ok2' :
+   forall (s : t) {Hs : Ok s} (f : elt -> bool)(x:elt),
+    In x (snd (partition f s)) -> In x s.
+  Proof.
+  induction s; simpl; auto; intros. inv.
+  generalize (IHs H1 f x).
+  destruct (f a); destruct (partition f s); simpl in *; auto.
+  inversion_clear H; auto.
+  Qed.
+  *)
+
+  Global Instance partition_ok1 : forall s f `(Ok s), Ok (fst (partition f s)).
+  Admitted.
+  (*
+  Proof.
+  simple induction s; simpl.
+  auto.
+  intros x l Hrec f Hs; inv.
+  generalize (@partition_ok1' _ _ f x).
+  generalize (Hrec f H0).
+  case (f x); case (partition f l); simpl; constructors; auto.
+  Qed.
+  *)
+
+  Global Instance partition_ok2 : forall s f `(Ok s), Ok (snd (partition f s)).
+  Admitted.
+(*
+  Proof.
+  simple induction s; simpl.
+  auto.
+  intros x l Hrec f Hs; inv.
+  generalize (@partition_ok2' _ _ f x).
+  generalize (Hrec f H0).
+  case (f x); case (partition f l); simpl; constructors; auto.
+  Qed.
+*)
+
+  Lemma elements_spec1 : forall s k v,
+    InA (fun p1 p2 => X.eq (fst p1) (fst p2) /\ snd p1 = snd p2) (k, v) (elements s) <-> MapsTo k v s.
+  Admitted.
+
+  Lemma elements_spec2w : forall s,
+     NoDupA  (fun p1 p2 => X.eq (fst p1) (fst p2) /\ snd p1 = snd p2) (@elements A s).
+  Admitted.
+
+  Lemma choose_spec1 : forall s k v,
+     choose s = Some (k,v) -> MapsTo k v s.
+  Admitted.
+
+  Lemma choose_spec2 : forall s , choose s = None -> Empty s.
+  Admitted.
+
+
+
+  (* Definition In := InA X.eq. *)
+  Definition eq := Equal.
+  Instance eq_equiv : Equivalence eq := _. Admitted.
+  End ForNotations.
+End MakeRaw.
+
+(** * Encapsulation
+
+   Now, in order to really provide a functor implementing [S], we
+   need to encapsulate everything into a type of lists without redundancy. *)
+
+Module Make (X: DecidableType) <: WMaps with Module E := X.
+ Module Raw := MakeRaw X.
+ Include WRaw2Maps X Raw.
+End Make.
+
